\section{Le 1.3}
Show that the observability gramian $\Sigma_o$ satisfies the Lyapunov equation
\begin{align*}
    A^T\,\Sigma_o + \Sigma_o\,A + C^T\,C = 0,
\end{align*}
or, 
\begin{align*}
    A^T\,\Sigma_o + \Sigma_o\,A = - C^T\,C.
\end{align*}
Multiply $e^{At}$ to the right and $e^{A^Tt}$ to the left,
\begin{align*}
    e^{A^Tt}\,A^T\,\Sigma_o\,e^{At} + e^{A^Tt}\,\Sigma_o\,A\,e^{At} = -e^{A^Tt}\,C^T\,C\,e^{At}.
\end{align*}
Since, 
\begin{align*}
    \frac{d}{dt}e^{At} = A\,e^{At}
\end{align*}
as $e^{At}$ and $A$ are commutative, 
\begin{align*}
    \left(\frac{d}{dt}e^{A^Tt}\right)\,\Sigma_o\,e^{At} + e^{A^Tt}\,\Sigma_o\,\left(\frac{d}{dt}e^{At}\right) = -e^{A^Tt}\,C^T\,C\,e^{At}.
\end{align*}
Using the product rule, 
\begin{align*}
    \frac{d}{dt}\left(e^{A^Tt}\,\Sigma_o\,e^{At}\right) = -e^{A^Tt}\,C^T\,C\,e^{At}.
\end{align*}
integrating both sides with limits from 0 to $\infty$
\begin{align*}
    \int_0^\infty\frac{d}{dt}\left(e^{A^Tt}\,\Sigma_o\,e^{At}\right) dt &= \int_0^\infty-e^{A^Tt}\,C^T\,C\,e^{At} dt.\\
    \implies \left[e^{A^Tt}\,\Sigma_o\,e^{At}\right]_0^\infty &= \int_0^\infty-e^{A^Tt}\,C^T\,C\,e^{At} dt.
\end{align*}
for a linear system with the state equation $\dot X = A\,X$ solves to $X = e^{At}$ and 
\begin{align*}
    \lim_{t\to\infty}X = \lim_{t\to\infty}e^{At} = 0
\end{align*}
if the eigenvalues are on the left-hand side of the complex plane.
Using the stability requirement
\begin{align*}
    \left[e^{A^Tt}\,\Sigma_o\,e^{At}\right]_0^\infty &= \int_0^\infty-e^{A^Tt}\,C^T\,C\,e^{At} dt.\\
    \text{becomes, } \Sigma_o &= \int_0^\infty e^{A^Tt}\,C^T\,C\,e^{At} dt.
\end{align*}